steel/Veritas.Steel.HashAccumulator.fst
@@ -1,0 +1,409 @@
+module Veritas.Steel.HashAccumulator
+module U8 = FStar.UInt8
+module U32 = FStar.UInt32
+module A = Veritas.Steel.Array
+
+open Steel.Memory
+open Steel.Effect.Common
+open Steel.Effect
+open Steel.Reference
+module AT = Steel.Effect.Atomic
+module Blake = Hacl.Blake2b_32
+
+let nat_at_most (f:U32.t) = x:nat{ x <= U32.v f }
+let u32_between (s f:U32.t) = x:U32.t { U32.v s <= U32.v x /\ U32.v x < U32.v f}
+
+let rec for_loop (start:U32.t)
+                 (finish:U32.t { U32.v start <= U32.v finish })
+                 (inv: nat -> vprop)
+                 (body:
+                    (i:u32_between start finish ->
+                          SteelT unit
+                          (inv (U32.v i))
+                          (fun _ -> inv (U32.v i + 1))))
+  : SteelT unit
+      (inv (U32.v start))
+      (fun _ -> inv (U32.v finish))
+  = if start = finish then (
+       AT.change_equal_slprop (inv _) (inv _);
+       AT.return ()
+    )
+    else (
+      body start;
+      let start' = U32.(start +^ 1ul) in
+      AT.change_equal_slprop (inv _) (inv (U32.v start'));
+      for_loop start' finish inv body;
+      AT.return ()
+    )
+
+assume
+val for_loop' (start:U32.t)
+             (finish:U32.t { U32.v start <= U32.v finish })
+             (inv: nat_at_most finish -> vprop)
+             (body:
+                    (i:u32_between start finish ->
+                          SteelT unit
+                          (inv (U32.v i))
+                          (fun _ -> inv (U32.v i + 1))))
+  : SteelT unit
+      (inv (U32.v start))
+      (fun _ -> inv (U32.v finish))
+
+let initial_hash
+  = Seq.create 32 0uy
+
+let hash_value (s:Seq.seq U8.t { Seq.length s <= blake2_max_input_length })
+  : hash_value_t
+  = Blake.spec s 0 Seq.empty 32
+
+noextract inline_for_extraction
+let xor_bytes (s1: Seq.seq U8.t)
+              (s2: Seq.seq U8.t { Seq.length s1 == Seq.length s2 })
+  : s3:Seq.seq U8.t { Seq.length s3 == Seq.length s1 }
+  = Seq.init (Seq.length s1)
+             (fun i -> Seq.index s1 i `FStar.UInt8.logxor` Seq.index s2 i)
+
+let elseq a (n:nat) = Ghost.erased (Seq.lseq a n)
+let elbytes n = elseq U8.t n
+
+let exor_bytes #l (s1 s2:elbytes l)
+  : elbytes l
+  = xor_bytes s1 s2
+
+let aggregate_hash_value (h0 h1: hash_value_t)
+  : hash_value_t
+  = xor_bytes h0 h1
+
+let state = a:A.array U8.t{ A.length a == 32 }
+
+[@@__steel_reduce__;__reduce__]
+let invariant (s:state) = A.varray s
+
+let v_hash
+     (#p:vprop)
+     (t:state)
+     (h:rmem p{
+       FStar.Tactics.with_tactic
+         selector_tactic
+         (can_be_split p (A.varray t) /\ True)
+     })
+  : GTot hash_value_t
+  = A.asel t h
+
+let create_in (_:unit)
+  = A.malloc 0uy 32ul
+open FStar.Ghost
+
+let exor_bytes_pfx #l (s1 s2:elbytes l) (i:nat { i <= l })
+  : elbytes l
+  = Seq.append
+      (exor_bytes #i (Seq.slice s1 0 i) (Seq.slice s2 0 i))
+      (Seq.slice s1 i (Seq.length s1))
+
+assume
+val varray_pts_to (#t:Type) (a:A.array t) (x:elseq t (A.length a)) : vprop
+
+assume
+val intro_varray_pts_to (#t:_)
+                        (#opened:inames)
+                        (a:A.array t)
+  : AT.SteelGhost (elseq t (A.length a)) opened
+    (A.varray a)
+    (fun x -> varray_pts_to a x)
+    (requires fun _ -> True)
+    (ensures fun h0 x h1 ->
+      Ghost.reveal x == A.asel a h0)
+
+assume
+val elim_varray_pts_to (#t:_)
+                       (#opened:inames)
+                       (a:A.array t)
+                       (c:elseq t (A.length a))
+  : AT.SteelGhost unit opened
+    (varray_pts_to a c)
+    (fun _ -> A.varray a)
+    (requires fun _ -> True)
+    (ensures fun _ _ h1 ->
+      A.asel a h1 == Ghost.reveal c)
+
+assume
+val read_pt (#t:_)
+            (a:A.array t)
+            (#r:elseq t (A.length a))
+            (i:U32.t { U32.v i < A.length a })
+  : Steel t
+    (varray_pts_to a r)
+    (fun _ -> varray_pts_to a r)
+    (requires fun _ -> True)
+    (ensures fun h0 v h1 ->
+      v == Seq.index r (U32.v i))
+
+assume
+val write_pt (#t:_)
+            (a:A.array t)
+            (#r:elseq t (A.length a))
+            (i:U32.t { U32.v i < A.length a })
+            (v:t)
+  : SteelT unit
+    (varray_pts_to a r)
+    (fun _ -> varray_pts_to a (Seq.upd r (U32.v i) v))
+
+let ehash_value_t = elbytes 32
+let upd_ehash_value (x:ehash_value_t) (i:nat{i < 32}) (v:U8.t)
+  : ehash_value_t
+  = Seq.upd x i v
+
+let extend_ehash_value (s1 s2:ehash_value_t) (i:nat { i < 32 })
+  : Lemma (upd_ehash_value
+                     (exor_bytes_pfx s1 s2 i)
+                     i
+                     (U8.logxor (Seq.index s1 i) (Seq.index s2 i)) `Seq.equal`
+           exor_bytes_pfx s1 s2 (i + 1))
+  = ()
+
+let hpts_to (x:hash_value_buf) (s:ehash_value_t) =
+  varray_pts_to x s
+
+let read_hbuf (#s:ehash_value_t) (x:hash_value_buf) (i:U32.t{U32.v i < 32})
+  : Steel U8.t
+    (hpts_to x s)
+    (fun _ -> hpts_to x s)
+    (requires fun _ -> True)
+    (ensures fun _ v _ ->
+      v == Seq.index s (U32.v i))
+  = let v = read_pt x i in AT.return v
+
+let write_hbuf (#s:ehash_value_t) (x:hash_value_buf) (i:U32.t{U32.v i < 32}) (v:U8.t)
+  : SteelT unit
+    (hpts_to x s)
+    (fun _ -> hpts_to x (upd_ehash_value s (U32.v i) v))
+  = write_pt x i v;
+    AT.change_equal_slprop (varray_pts_to _ _)
+                           (hpts_to _ _)
+
+let intro_hpts_to (#o:_) (x:hash_value_buf)
+  : AT.SteelGhost ehash_value_t o
+    (A.varray x)
+    (fun v -> hpts_to x v)
+    (requires fun _ -> True)
+    (ensures fun h v _ ->
+      as_hash_value x h == Ghost.reveal v)
+  = intro_varray_pts_to x
+
+let elim_hpts_to (#o:_) (#e:ehash_value_t) (x:hash_value_buf)
+  : AT.SteelGhost unit o
+    (hpts_to x e)
+    (fun _ -> A.varray x)
+    (requires fun _ -> True)
+    (ensures fun _ _ h ->
+      Ghost.reveal e == as_hash_value x h)
+  = elim_varray_pts_to x e
+
+#push-options "--query_stats --fuel 0 --ifuel 0"
+let aggregate_hash_value_pts
+    (s1: ehash_value_t)
+    (s2: ehash_value_t)
+    (b1: hash_value_buf)
+    (b2: hash_value_buf)
+  : SteelT unit
+    (hpts_to b1 s1 `star`
+     hpts_to b2 s2)
+    (fun _ ->
+     hpts_to b1 (exor_bytes s1 s2) `star`
+     hpts_to b2 s2)
+  = let inv (i:nat_at_most 32ul)
+      : vprop
+      = hpts_to b1 (exor_bytes_pfx s1 s2 i) `star`
+        hpts_to b2 s2
+    in
+    let body (i:u32_between 0ul 32ul)
+      : SteelT unit
+        (inv (U32.v i))
+        (fun _ -> inv (U32.v i + 1))
+      = AT.change_equal_slprop
+            (inv (U32.v i))
+            (hpts_to b1 (exor_bytes_pfx s1 s2 (U32.v i)) `star`
+             hpts_to b2 s2);
+        let x1 = read_hbuf b1 i in
+        let x2 = read_hbuf b2 i in
+        write_hbuf b1 i (U8.logxor x1 x2);
+        AT.slassert (hpts_to b1 (upd_ehash_value
+                                          (exor_bytes_pfx s1 s2 (U32.v i))
+                                          (U32.v i)
+                                          (U8.logxor x1 x2)));
+        extend_ehash_value s1 s2 (U32.v i);
+        AT.change_equal_slprop (hpts_to b1 _)
+                               (hpts_to b1 (exor_bytes_pfx s1 s2 (U32.v i + 1)));
+        AT.change_equal_slprop (hpts_to b1 _ `star` hpts_to b2 _)
+                               (inv (U32.v i + 1));
+        AT.return ()
+    in
+    assert (exor_bytes_pfx s1 s2 0 `Seq.equal` s1);
+    AT.change_equal_slprop (hpts_to b1 _ `star` hpts_to b2 _)
+                           (inv 0);
+    for_loop' 0ul 32ul inv body;
+    assert (exor_bytes_pfx s1 s2 32 `Seq.equal` exor_bytes s1 s2);
+    AT.change_equal_slprop (inv 32)
+                           (hpts_to b1 _ `star` hpts_to b2 _);
+    AT.return ()
+
+let aggregate_hash_value_buf (b1: hash_value_buf) (b2: hash_value_buf)
+  = let _ = intro_hpts_to b1 in
+    let _ = intro_hpts_to b2 in
+    aggregate_hash_value_pts _ _ b1 b2;
+    elim_hpts_to b1;
+    elim_hpts_to b2
+
+
+let size_t = U32.t
+let max_output = 64
+
+assume
+val blake2b:
+    nn:size_t{1 <= UInt32.v nn /\ UInt32.v nn <= max_output}
+  -> output: A.array U8.t
+  -> ll: size_t
+  -> d: A.array U8.t
+  -> Steel unit
+  (A.varray output `star` A.varray d)
+  (fun _ -> A.varray output `star` A.varray d)
+  (requires fun _ ->
+    A.length d >= U32.v ll /\
+    A.length output = U32.v nn)
+  (ensures fun h0 _ h1 ->
+    A.length d >= U32.v ll /\
+    A.length output = U32.v nn /\
+    A.asel d h0 == A.asel d h1 /\
+    A.asel output h1 ==
+      Blake.spec
+        (Seq.slice (A.asel d h0) 0 (U32.v ll))
+        0 Seq.empty (UInt32.v nn))
+
+let add' (s:hash_value_buf) (input:hashable_buffer) (l:U32.t)
+  : Steel unit
+    (A.varray s `star` A.varray input)
+    (fun _ -> A.varray s `star` A.varray input)
+    (requires fun h0 ->
+      U32.v l <= A.length input)
+    (ensures fun h0 _ h1 ->
+      U32.v l <= A.length input /\
+      A.asel s h1 ==
+      aggregate_hash_value (A.asel s h0)
+                           (hash_value (Seq.slice (A.asel input h0) 0 (U32.v l))))
+  = let tmp = A.malloc 0uy 32ul in
+    blake2b 32ul tmp l input;
+    aggregate_hash_value_buf s tmp;
+    A.free tmp;
+    AT.return ()
+
+let add (s:state) (input:hashable_buffer) (l:U32.t) =
+  add' s input l; AT.sladmit()
+
+
+(* Crashes F* *)
+// let for_loop (start:U32.t)
+//              (finish:U32.t)
+//              (inv: nat -> vprop)
+//              (body:
+//              (i:U32.t ->
+//                    Steel unit
+//                    (inv (U32.v i))
+//                    (fun _ -> inv (U32.v i + 1))
+//                    (requires fun _ -> U32.v start <= U32.v i /\
+//                                    U32.v start < U32.v finish)
+//                    (ensures fun _ _ _ -> True)))
+//   : Steel unit
+//       (inv (U32.v start))
+//       (fun _ -> inv (U32.v finish))
+//       (requires fun _ ->
+//         U32.v start <= U32.v finish)
+//       (ensures fun _ _ _ ->
+//         True)
+//   = let rec aux (i:U32.t)
+//       : Steel unit
+//         (inv (U32.v i))
+//         (fun _ -> inv (U32.v finish))
+//         (requires fun _ ->
+//           U32.v start <= U32.v i /\
+//           U32.v i <= U32.v finish)
+//         (ensures fun _ _ _ -> True)
+//       = AT.sladmit(); AT.return ()
+//     in
+//     aux start
+
+let coerce #t (#l0 #l1:_) (e:elseq t l0 { l0 = l1}) : elseq t l1 = e
+
+let prefix_copied #t #l0 #l1
+                  (e0:elseq t l0)
+                  (e1:elseq t l1)
+                  (i:nat { i <= l0 /\ l0 == l1})
+   : elseq t l1
+   = (Seq.append (Seq.slice e0 0 i) (Seq.slice e1 i (Seq.length e1)))
+
+let slice_lem (#t:_)
+              (#l0 #l1:_)
+              (e0:elseq t l0)
+              (e1:elseq t l1)
+  : Lemma
+    (requires l0 == l1)
+    (ensures Seq.append (Seq.slice e0 0 l0)
+                        (Seq.slice e1 l0 l1) `Seq.equal`
+             coerce #t #l0 #l1 e0)
+  = ()
+
+let memcpy #t (a0 a1:A.array t)
+              (#e0:elseq t (A.length a0))
+              (#e1:elseq t (A.length a1))
+              (i:U32.t{ U32.v i == A.length a0 /\ A.length a0 == A.length a1 })
+  : SteelT unit
+    (varray_pts_to a0 e0 `star` varray_pts_to a1 e1)
+    (fun _ -> varray_pts_to a0 e0 `star` varray_pts_to a1 (coerce e0))
+  = let inv (j:nat_at_most i)
+      : vprop
+      = varray_pts_to a0 e0 `star`
+        varray_pts_to a1 (Seq.append (Seq.slice e0 0 j) (Seq.slice e1 j (Seq.length e1)))
+    in
+    let body (j:u32_between 0ul i)
+      : SteelT unit
+        (inv (U32.v j))
+        (fun _ -> inv (U32.v j + 1))
+      = // let z = read_pt a0 j in
+        // write_pt a1 j z;
+        AT.sladmit();
+        AT.return ()
+    in
+    assert (Seq.append (Seq.slice e0 0 0) (Seq.slice e1 0 (Seq.length e1)) `Seq.equal`
+            e1);
+    AT.change_equal_slprop (varray_pts_to a1 _)
+                           (varray_pts_to a1
+                             (Seq.append (Seq.slice e0 0 (U32.v 0ul))
+                                         (Seq.slice e1 (U32.v 0ul) (Seq.length e1))));
+    AT.change_equal_slprop (varray_pts_to a0 e0 `star` varray_pts_to a1 _)
+                           (inv (U32.v 0ul));
+    for_loop' 0ul i inv body;
+    AT.slassert (inv (U32.v i));
+    AT.change_equal_slprop (inv (U32.v i))
+                           (varray_pts_to a0 e0 `star`
+                            varray_pts_to a1
+                             (Seq.append (Seq.slice e0 0 (U32.v i))
+                                         (Seq.slice e1 (U32.v i) (Seq.length e1))));
+    slice_lem e0 e1;
+    AT.change_equal_slprop (varray_pts_to a1
+                                          (Seq.append (Seq.slice e0 0 (U32.v i))
+                                          (Seq.slice e1 (U32.v i) (Seq.length e1))))
+                           (varray_pts_to a1 (coerce e0));
+    AT.return ()
+
+let get' (#e0 #e1:ehash_value_t)
+         (s:state)
+         (out:hash_value_buf)
+  : Steel unit
+    (hpts_to s `star` A.varray out)
+    (fun _ -> invariant s `star` A.varray out)
+    (requires fun h0 -> True)
+    (ensures fun h0 r h1 ->
+      v_hash s h0 == as_hash_value out h1)
+
+//     (
+let as_hash_value_pfx (b:hash_value_buf) (h:HS.mem) (n:nat { n <= 32 }) =
+  Seq.slice (as_hash_value b h) 0 n
