steel/Veritas.Steel.HashAccumulator.fsti
@@ -1,0 +1,100 @@
+module Veritas.Steel.HashAccumulator
+module U8 = FStar.UInt8
+module U32 = FStar.UInt32
+module A = Steel.Array
+
+open Steel.Effect.Common
+open Steel.Effect
+open Steel.Reference
+
+inline_for_extraction noextract
+let blake2_max_input_length = pow2 32 - 1 - 128
+
+// NOTE: we do not have an agile spec for the keyed hash functionality :(, so
+// we're making Blake2-dependent assumptions without corresponding agile predicates
+noextract inline_for_extraction
+let hashable_bytes = s:Seq.seq U8.t { Seq.length s <= blake2_max_input_length }
+let hashable_buffer = b:A.array U8.t { A.length b <= blake2_max_input_length }
+
+let hash_value_t = Seq.lseq U8.t 32
+
+val initial_hash
+  : hash_value_t
+
+val hash_value (_:hashable_bytes)
+  : hash_value_t
+
+val aggregate_hash_value (_ _: hash_value_t)
+  : hash_value_t
+
+let hash_value_buf = b:A.array U8.t{ A.length b == 32 }
+
+[@@ __steel_reduce__]
+let as_hash_value (#p:vprop) (r:hash_value_buf)
+    (h:rmem p{FStar.Tactics.with_tactic selector_tactic (can_be_split p (A.varray r) /\ True)})
+  = A.asel r h
+
+val state : Type0
+
+val invariant (s: state) : vprop
+
+val v_hash
+     (#p:vprop)
+     (t:state)
+     (h:rmem p{
+       FStar.Tactics.with_tactic
+         selector_tactic
+         (can_be_split p (invariant t) /\ True)
+     })
+  : GTot hash_value_t
+
+
+(*** THE MAIN INTERFACE ***)
+
+(** Create an instance of a hash accumulator in the heap *)
+val create_in (_:unit)
+  : Steel state
+    emp
+    (fun s -> invariant s)
+    (requires fun _ -> True)
+    (ensures fun _ s h1 ->
+       v_hash s h1 == initial_hash)
+
+(** Combine two hash values held in b1 and b2 into b1 *)
+val aggregate_hash_value_buf (b1: hash_value_buf) (b2: hash_value_buf)
+  : Steel unit
+    (A.varray b1 `star` A.varray b2)
+    (fun _ -> A.varray b1 `star` A.varray b2)
+    (requires fun _ -> True)
+    (ensures fun h0 _ h1 ->
+      as_hash_value b2 h0 == as_hash_value b2 h1 /\
+      as_hash_value b1 h1 == aggregate_hash_value (as_hash_value b1 h0)
+                                                  (as_hash_value b2 h0))
+
+(** Hash the (input[0, l)) into the hash accumulate s *)
+val add (s:state) (input:hashable_buffer) (l:U32.t)
+  : Steel unit
+    (invariant s `star` A.varray input)
+    (fun _ -> invariant s `star` A.varray input)    
+    (requires fun h0 ->
+      U32.v l <= A.length input)
+    (ensures fun h0 _ h1 ->
+      U32.v l <= A.length input /\    
+      v_hash s h1 ==
+      aggregate_hash_value (v_hash s h0)
+                           (hash_value (Seq.slice (A.asel input h0) 0 (U32.v l))))
+
+(** Read the current value of the hash into out *)
+val get (s:state) (out:hash_value_buf)
+  : Steel unit
+    (invariant s `star` A.varray out)
+    (fun _ -> invariant s `star` A.varray out)
+    (requires fun h0 -> True)
+    (ensures fun h0 r h1 ->
+      v_hash s h0 == as_hash_value out h1)
+
+(** Free the hash accumulator *)
+val free (s:state)
+  : SteelT unit
+    (invariant s)
+    (fun _ -> emp)
